Add comments to lemmas and functions in Sets.dfy

Sets/Sets.dfy
@@ -3,6 +3,10 @@ include "../Mathematics.dfy"
 module Sets {
   import Math = Mathematics
 
+  /**
+   * If x is a proper subset of y, then the cardinality of x is less than
+   * the cardinality of y.
+   */
   lemma lemma_proper_subset_cardinality<T>(x: set<T>, y: set<T>)
     requires x < y
     ensures |x| < |y|
@@ -14,6 +18,10 @@ module Sets {
     }
   }
 
+  /**
+   * If x is a subset of y, then the cardinality of x is less than or equal to
+   * the cardinality of y.
+   */
   lemma lemma_subset_cardinality<T>(x: set<T>, y: set<T>)
     ensures x < y ==> |x| < |y|
     ensures x == y ==> |x| == |y|
@@ -24,6 +32,10 @@ module Sets {
     }
   }
 
+  /**
+   * If x is a subset of y and the cardinality of x is equal to the cardinality
+   * of y, x is equal to y.
+   */
   lemma lemma_subset_equality<T>(x: set<T>, y: set<T>)
     requires x <= y
     requires |x| == |y|
@@ -37,12 +49,18 @@ module Sets {
     }
   }
 
+  /**
+   * A singleton set has a cardinality of 1.
+   */
   lemma lemma_singleton_set_cardinality<T>(x: set<T>, e: T)
     requires x == {e}
     ensures |x| == 1
   {
   }
 
+  /**
+   * Elements in a singleton set are equal to each other.
+   */
   lemma lemma_singleton_set_equality<T>(foo: set<T>, x: T, y: T)
     requires |foo| == 1
     requires x in foo
@@ -58,6 +76,10 @@ module Sets {
     }
   }
 
+  /**
+   * If an injective function is applied to each element of a set to construct
+   * another set, the two sets have the same cardinality. 
+   */
   lemma lemma_map_set_to_set_cardinality<X, Y>(xs: set<X>, ys: set<Y>, f: X-->Y)
     requires forall x :: f.requires(x)
     requires Math.injective(f)
@@ -75,6 +97,9 @@ module Sets {
     }
   }
 
+  /**
+   * Apply an injective function to each element of a set.
+   */
   function method {:opaque} map_set_to_set<X(!new), Y>(xs: set<X>, f: X-->Y): set<Y>
     reads f.reads
     requires forall x :: f.requires(x)
@@ -87,6 +112,9 @@ module Sets {
     ys
   }
 
+  /**
+   * Apply an injective function to each element of a sequence.
+   */
   function method {:opaque} map_seq_to_set<X(!new), Y>(xs: seq<X>, f: X-->Y): set<Y>
     reads f.reads
     requires forall x :: f.requires(x)
@@ -97,6 +125,11 @@ module Sets {
     if |xs| == 0 then {} else map_seq_to_set(xs[1..], f) + {f(xs[0])}
   }
 
+  /**
+   * If a set ys is constructed using elements of another set xs for which a
+   * function returns true, the cardinality of ys is less than or equal to the
+   * cardinality of xs.
+   */
   lemma lemma_filter_cardinality<X>(xs: set<X>, ys: set<X>, f: X~>bool)
     requires forall x :: x in xs ==> f.requires(x)
     requires forall y :: y in ys ==> y in xs && f(y)
@@ -112,6 +145,10 @@ module Sets {
     }
   }
 
+  /**
+   * Construct a set using elements of another set for which a function returns
+   * true.
+   */
   function method {:opaque} filter<X(!new)>(xs: set<X>, f: X~>bool): set<X>
     reads f.reads
     requires forall x :: x in xs ==> f.requires(x)
@@ -123,9 +160,13 @@ module Sets {
     ys
   }
 
+  /**
+   * The cardinality of a union of two sets greater than either individual set.
+   */
   lemma lemma_union_cardinality<X>(xs: set<X>, ys: set<X>, us: set<X>)
     requires us == xs + ys
     ensures |us| >= |xs|
+    ensures |us| >= |ys|
     decreases ys
   {
     if ys == {} {
@@ -144,23 +185,29 @@ module Sets {
     }
   }
 
-  function method set_of_numbers_in_right_exclusive_range(a: int, b: int): set<int>
+  /**
+   * Construct a set containing all integers in the range [a, b).
+   */
+  function method set_range(a: int, b: int): set<int>
     requires a <= b
     ensures forall i :: a <= i < b <==> i
-            in set_of_numbers_in_right_exclusive_range(a, b)
-    ensures |set_of_numbers_in_right_exclusive_range(a, b)| == b - a
+            in set_range(a, b)
+    ensures |set_range(a, b)| == b - a
     decreases b - a
   {
-    if a == b then {}
-    else {a} + set_of_numbers_in_right_exclusive_range(a + 1, b)
+    if a == b then {} else {a} + set_range(a + 1, b)
   }
 
+  /**
+   * If a set solely contains integers in the range [a, b) then its cardinality
+   * is bounded by b - a.
+   */
   lemma lemma_bounded_set_cardinality(x: set<int>, a: int, b: int)
     requires forall i :: i in x ==> a <= i < b
     requires a <= b
     ensures |x| <= b - a
   {
-    var range := set_of_numbers_in_right_exclusive_range(a, b);
+    var range := set_range(a, b);
     forall e | e in x
       ensures e in range;
     {
@@ -169,28 +216,37 @@ module Sets {
     lemma_subset_cardinality(x, range);
   }
 
-  function set_range(n: int): set<int>
+  /**
+   * Construct a set containing all integers in the range [0, n).
+   */
+  function set_range_zero_bound(n: int): set<int>
     requires n >= 0
-    ensures forall i :: 0 <= i < n <==> i in set_range(n)
-    ensures |set_range(n)| == n
+    ensures forall i :: 0 <= i < n <==> i in set_range_zero_bound(n)
+    ensures |set_range_zero_bound(n)| == n
     decreases n
   {
-    if n == 0 then {}
-    else {n - 1} + set_range(n - 1)
+    if n == 0 then {} else {n - 1} + set_range_zero_bound(n - 1)
   }
 
+  /**
+   * If a set contains all integers in the range [0, n) then its cardinality is
+   * n.
+   */
   lemma {:induction n} lemma_set_range_cardinality(n: int)
     requires n >= 0
-    ensures |set_range(n)| == n
+    ensures |set_range_zero_bound(n)| == n
     decreases n
   {
     if n == 0 {
     } else {
       lemma_set_range_cardinality(n - 1);
-      assert set_range(n) == set_range(n - 1) + {n - 1};
+      assert set_range_zero_bound(n) == set_range_zero_bound(n - 1) + {n - 1};
     }
   }
 
+  /**
+   * If all elements in set x are in set y, x is a subset of y.
+   */
   lemma lemma_subset_extensionality<T>(x: set<T>, y: set<T>)
     requires forall e | e in x :: e in y
     ensures x <= y
